hol/symb_exec/p4_symb_execLib.sig
@@ -2,6 +2,10 @@ signature p4_symb_execLib =
 sig
   include Abbrev
 
+datatype defn_data =
+   def_term of term
+ | def_thm of thm;
+
 val p4_symb_exec:
    int ->
    bool ->
@@ -17,17 +21,17 @@ val p4_symb_exec:
 val p4_symb_exec_prove_contract:
    bool ->
    hol_type ->
-     term -> (term * term * term) -> string list -> thm list -> term -> term list -> term list -> thm list -> thm -> (thm -> bool) option -> int -> term -> thm
+     defn_data -> (term * term * term) -> string list -> thm list -> term -> term list -> term list -> thm list -> thm -> (thm -> bool) option -> int -> term -> thm list -> thm
 
 val p4_symb_exec_prove_contract_conc:
    bool ->
    hol_type ->
-     term -> (term * term * term) -> string list -> thm list ->
-       term -> term list -> term list -> thm list -> thm -> (thm -> bool) option -> int -> term -> thm
+     defn_data -> (term * term * term) -> string list -> thm list ->
+       term -> term list -> term list -> thm list -> thm -> (thm -> bool) option -> int -> term -> thm list -> thm
 
 val p4_debug_symb_exec:
    hol_type ->
-     term ->
+     defn_data ->
        (term * term * term) -> 
          string list -> thm list ->
 	   term ->
@@ -41,11 +45,15 @@ val p4_debug_symb_exec:
 
 val p4_debug_symb_exec_frame_lists:
    hol_type ->
-     term ->
+     defn_data ->
        (term * term * term) ->
          string list -> thm list ->
 	   term ->
 	     term list ->
 	       term list -> thm list -> thm -> int -> symb_execLib.path_tree * term list
+
+val get_v1model_wellformed_defs : term -> term -> Defn.defn
+
+val p4_combine_contracts: thm -> thm -> thm -> thm
 
 end
