hol/symb_exec/p4_symb_exec_test7Script.sml
@@ -290,12 +290,12 @@ val p4_is_finished_alt_opt = NONE
 val n_max = 150;
 val postcond = “(\s. T):v1model_ascope astate -> bool”;
 val fuel = 1;
-
+val postcond_rewr_thms = []
 
 val time_start = Time.now(); (*
 val p4_symb_exec_fun = (p4_symb_exec 1)
 *)
-val contract_thm = p4_symb_exec_prove_contract debug_flag arch_ty ctx (fty_map, b_fty_map, pblock_action_names_map) const_actions_tables path_cond_defs init_astate stop_consts_rewr stop_consts_never [] path_cond p4_is_finished_alt_opt n_max postcond;
+val contract_thm = p4_symb_exec_prove_contract debug_flag arch_ty (def_term ctx) (fty_map, b_fty_map, pblock_action_names_map) const_actions_tables path_cond_defs init_astate stop_consts_rewr stop_consts_never [] path_cond p4_is_finished_alt_opt n_max postcond postcond_rewr_thms;
 
 val _ = print (String.concat ["Total time consumption: ",
                               (LargeInt.toString $ Time.toMilliseconds ((Time.now()) - time_start)),
