hol/symb_exec/p4_symb_exec_test3Script.sml
@@ -160,6 +160,7 @@ val path_cond = ASSUME “e8 = T”
 val p4_is_finished_alt_opt = NONE
 val n_max = 50;
 val postcond = “(\s. packet_has_port s 1):v1model_ascope astate -> bool”;
+val postcond_rewr_thms = [p4_symb_execTheory.packet_has_port_def]
 (* For debugging:
 val comp_thm = INST_TYPE [Type.alpha |-> arch_ty] p4_exec_semTheory.arch_multi_exec_comp_n_tl_assl
 *)
@@ -176,6 +177,6 @@ val [(path_cond_res, step_thm), (path_cond2_res, step_thm2)] =
 
 (* Finishes at 45 steps (one step of which is a symbolic branch)
  * (higher numbers as arguments will work, but do no extra computations) *)
-val contract_thm = p4_symb_exec_prove_contract_conc debug_flag arch_ty ctx (fty_map, b_fty_map, pblock_action_names_map) const_actions_tables path_cond_defs init_astate stop_consts_rewr stop_consts_never [] path_cond p4_is_finished_alt_opt n_max postcond;
+val contract_thm = p4_symb_exec_prove_contract_conc debug_flag arch_ty (def_term ctx) (fty_map, b_fty_map, pblock_action_names_map) const_actions_tables path_cond_defs init_astate stop_consts_rewr stop_consts_never [] path_cond p4_is_finished_alt_opt n_max postcond postcond_rewr_thms;
 
 val _ = export_theory ();
